POC: Folding of algebraic zeros in value analysis
The function
```
int f(int x, int y) {
    int z = 0;
    return x | (y * z);
}
```
always returns `x`, neither the multiplication nor the bitwise-or is needed.
CompCert removes the multiplication (replacing it by loading 0 into a
register), but leaves the or operation.

The reason for this is that the replacement of `y * 0` by 0 only takes place
at the "strength reduction" stage, which is purely local to the current
operation. Values are propagated before, by the value analysis, but the
value analysis does not contain a rule for folding this expression. Indeed,
it cannot represent this, because the value of `y` may be `Vundef`, and the
value domain's notion of "match" does not allow us to replace an undefined
value by the more defined constant 0.

This patch extends the value domain with a new constructor `Ix` (integer or
don't care, i.e., undefined) and adds just enough machinery to allow us to
handle the above example program correctly. As this involves a nontrivial
amount of code duplication, even just to handle the bitwise-or operator, it
is clearly not the best approach for doing this.

backend/ValueDomain.v
@@ -528,6 +528,7 @@ Qed.
 Inductive aval : Type :=
   | Vbot                     (**r bottom (empty set of values) *)
   | I (n: int)               (**r exactly [Vint n] *)
+  | Ix (n: int)              (**r exactly [Vint n], or [Vundef] *)
   | Uns (p: aptr) (n: Z)     (**r a [n]-bit unsigned integer, or [Vundef] *)
   | Sgn (p: aptr) (n: Z)     (**r a [n]-bit signed integer, or [Vundef] *)
   | L (n: int64)             (**r exactly [Vlong n] *)
@@ -559,6 +560,8 @@ Definition is_sgn (n: Z) (i: int) : Prop :=
 
 Inductive vmatch : val -> aval -> Prop :=
   | vmatch_i: forall i, vmatch (Vint i) (I i)
+  | vmatch_ix: forall i, vmatch (Vint i) (Ix i)
+  | vmatch_ix_undef: forall i, vmatch Vundef (Ix i)
   | vmatch_Uns: forall p i n, 0 <= n -> is_uns n i -> vmatch (Vint i) (Uns p n)
   | vmatch_Uns_undef: forall p n, vmatch Vundef (Uns p n)
   | vmatch_Sgn: forall p i n, 0 < n -> is_sgn n i -> vmatch (Vint i) (Sgn p n)
@@ -815,18 +818,22 @@ Qed.
 Inductive vge: aval -> aval -> Prop :=
   | vge_bot: forall v, vge v Vbot
   | vge_i: forall i, vge (I i) (I i)
+  | vge_ix: forall i, vge (Ix i) (Ix i)
   | vge_l: forall i, vge (L i) (L i)
   | vge_f: forall f, vge (F f) (F f)
   | vge_s: forall f, vge (FS f) (FS f)
   | vge_uns_i: forall p n i, 0 <= n -> is_uns n i -> vge (Uns p n) (I i)
+  | vge_uns_ix: forall p n i, 0 <= n -> is_uns n i -> vge (Uns p n) (Ix i)
   | vge_uns_uns: forall p1 n1 p2 n2, n1 >= n2 -> pge p1 p2 -> vge (Uns p1 n1) (Uns p2 n2)
   | vge_sgn_i: forall p n i, 0 < n -> is_sgn n i -> vge (Sgn p n) (I i)
+  | vge_sgn_ix: forall p n i, 0 < n -> is_sgn n i -> vge (Sgn p n) (Ix i)
   | vge_sgn_sgn: forall p1 n1 p2 n2, n1 >= n2 -> pge p1 p2 -> vge (Sgn p1 n1) (Sgn p2 n2)
   | vge_sgn_uns: forall p1 n1 p2 n2, n1 > n2 -> pge p1 p2 -> vge (Sgn p1 n1) (Uns p2 n2)
   | vge_p_p: forall p q, pge p q -> vge (Ptr p) (Ptr q)
   | vge_ip_p: forall p q, pge p q -> vge (Ifptr p) (Ptr q)
   | vge_ip_ip: forall p q, pge p q -> vge (Ifptr p) (Ifptr q)
   | vge_ip_i: forall p i, vge (Ifptr p) (I i)
+  | vge_ip_ix: forall p i, vge (Ifptr p) (Ix i)
   | vge_ip_l: forall p i, vge (Ifptr p) (L i)
   | vge_ip_f: forall p f, vge (Ifptr p) (F f)
   | vge_ip_s: forall p f, vge (Ifptr p) (FS f)
@@ -1580,11 +1587,22 @@ Proof.
 - inv H; inv H0; try (destruct (eq_block b b0)); eauto using psub_sound, poffset_sound, pmatch_lub_l with va.
 Qed.
 
-Definition mul := binop_int Int.mul.
+Definition mul (v w: aval) :=
+  match v, w with
+  | I i1, I i2 => I (Int.mul i1 i2)
+  | I i, _ | Ix i, _ => if Int.eq i Int.zero then Ix Int.zero else ntop1 w
+  | _, I i | _, Ix i => if Int.eq i Int.zero then Ix Int.zero else ntop1 v
+  | _, _ => ntop2 v w
+  end.
 
 Lemma mul_sound:
   forall v x w y, vmatch v x -> vmatch w y -> vmatch (Val.mul v w) (mul x y).
-Proof (binop_int_sound Int.mul).
+Proof.
+  intros. unfold Val.mul, mul.
+- inv H; inv H0; eauto with va;
+    (predSpec Int.eq Int.eq_spec i Int.zero; subst; constructor) ||
+    (predSpec Int.eq Int.eq_spec i0 Int.zero; subst; try rewrite Int.mul_zero; constructor).
+Qed.
 
 Definition mulhs := binop_int Int.mulhs.
 
@@ -2825,27 +2843,31 @@ Definition vnormalize (chunk: memory_chunk) (v: aval) :=
   match chunk, v with
   | _, Vbot => Vbot
   | Mint8signed, I i => I (Int.sign_ext 8 i)
+  | Mint8signed, Ix i => Ix (Int.sign_ext 8 i)
   | Mint8signed, Uns p n => if zlt n 8 then Uns (provenance v) n else Sgn (provenance v) 8
   | Mint8signed, Sgn p n => Sgn (provenance v) (Z.min n 8)
   | Mint8signed, _ => Sgn (provenance v) 8
   | Mint8unsigned, I i => I (Int.zero_ext 8 i)
+  | Mint8unsigned, Ix i => Ix (Int.zero_ext 8 i)
   | Mint8unsigned, Uns p n => Uns (provenance v) (Z.min n 8)
   | Mint8unsigned, _ => Uns (provenance v) 8
   | Mint16signed, I i => I (Int.sign_ext 16 i)
+  | Mint16signed, Ix i => Ix (Int.sign_ext 16 i)
   | Mint16signed, Uns p n => if zlt n 16 then Uns (provenance v) n else Sgn (provenance v) 16
   | Mint16signed, Sgn p n => Sgn (provenance v) (Z.min n 16)
   | Mint16signed, _ => Sgn (provenance v) 16
   | Mint16unsigned, I i => I (Int.zero_ext 16 i)
+  | Mint16unsigned, Ix i => Ix (Int.zero_ext 16 i)
   | Mint16unsigned, Uns p n => Uns (provenance v) (Z.min n 16)
   | Mint16unsigned, _ => Uns (provenance v) 16
-  | Mint32, (I _ | Uns _ _ | Sgn _ _ | Ifptr _) => v
+  | Mint32, (I _ | Ix _ | Uns _ _ | Sgn _ _ | Ifptr _) => v
   | Mint32, Ptr p => if Archi.ptr64 then Ifptr p else v
   | Mint64, (L _ | Ifptr _) => v
   | Mint64, (Uns p _ | Sgn p _) => Ifptr p
   | Mint64, Ptr p => if Archi.ptr64 then v else Ifptr p
   | Mfloat32, FS f => v
   | Mfloat64, F f => v
-  | Many32, (I _ | Uns _ _ | Sgn _ _ | FS _ | Ifptr _) => v
+  | Many32, (I _ | Ix _ | Uns _ _ | Sgn _ _ | FS _ | Ifptr _) => v
   | Many32, Ptr p => if Archi.ptr64 then Ifptr p else v
   | Many64, _ => v
   | _, _ => Ifptr (provenance v)
@@ -2942,10 +2964,24 @@ Proof with (auto using provenance_monotone with va).
   apply is_sign_ext_sgn...
 - constructor... apply is_zero_ext_uns... apply Z.min_case...
 - unfold provenance; destruct (va_strict tt)...
+- destruct (zlt n 8); constructor...
+  apply is_sign_ext_uns...
+  apply is_sign_ext_sgn...
+- constructor... apply is_zero_ext_uns... apply Z.min_case...
+- destruct (zlt n 16); constructor...
+  apply is_sign_ext_uns...
+  apply is_sign_ext_sgn...
+- constructor... apply is_zero_ext_uns... apply Z.min_case...
+- unfold provenance; destruct (va_strict tt)...
 - destruct (zlt n1 8). rewrite zlt_true by omega...
   destruct (zlt n2 8)...
 - destruct (zlt n1 16). rewrite zlt_true by omega...
   destruct (zlt n2 16)...
+- constructor... apply is_sign_ext_sgn... apply Z.min_case...
+- constructor... apply is_zero_ext_uns...
+- constructor... apply is_sign_ext_sgn... apply Z.min_case...
+- constructor... apply is_zero_ext_uns...
+- unfold provenance; destruct (va_strict tt)...
 - constructor... apply is_sign_ext_sgn... apply Z.min_case...
 - constructor... apply is_zero_ext_uns...
 - constructor... apply is_sign_ext_sgn... apply Z.min_case...
@@ -2959,6 +2995,11 @@ Proof with (auto using provenance_monotone with va).
 - destruct ptr64...
 - destruct ptr64...
 - destruct ptr64...
+- constructor... apply is_sign_ext_sgn...
+- constructor... apply is_zero_ext_uns...
+- constructor... apply is_sign_ext_sgn...
+- constructor... apply is_zero_ext_uns...
+- unfold provenance; destruct (va_strict tt)...
 - constructor... apply is_sign_ext_sgn...
 - constructor... apply is_zero_ext_uns...
 - constructor... apply is_sign_ext_sgn...
